\subsection{作业 4}

\begin{homework}
    写出函数
    \begin{align*}
        f(t) &= \begin{cases}
            \mathe^{-at}, & t > 0, \\
            0, & t \leq 0,
        \end{cases}
    \end{align*}
    的傅里叶变换，其中 $a > 0$。
\end{homework}

\begin{solution}
    \begin{align*}
        F(\omega) & = \int_{-\infty}^{+\infty}f(t)\mathe^{-\mathi\omega t}\D{t} \\
        & = \int_{0}^{+\infty}\mathe^{-at}\mathe^{-\mathi\omega t}\D{t} \\
        & = \int_{0}^{+\infty}\mathe^{-(a+\mathi\omega)t}\D{t} \\
        & = \left.\frac{\mathe^{-(a+\mathi\omega)t}}{-(a+\mathi\omega)}\right|_{0}^{+\infty} \\
        & = 0 - \frac{1}{-(a+\mathi\omega)} \\
        & = \frac{1}{a+\mathi\omega}.
    \end{align*}
    因此，$f(t)$ 的傅里叶变换为
    \begin{align*}
        F(\omega) = \frac{1}{a+\mathi\omega}.
    \end{align*}
\end{solution}

\begin{homework}
    已知
    \begin{align*}
        f(t) &= \begin{cases}
            t, & 0 \le t < \tau, \\
            \tau, & \tau \le t \le 2\tau, \\
            0, & t < 0 \text{ 或 } t > 2\tau,
        \end{cases}
    \end{align*}
    求 $f(t)$ 的傅里叶变换，其中 $\tau > 0$。
\end{homework}

\begin{solution}
    \begin{align*}
        F(\omega) & = \int_{-\infty}^{+\infty}f(t)\mathe^{-\mathi\omega t}\D{t} \\
        & = \int_{0}^{\tau}t\mathe^{-\mathi\omega t}\D{t} + \int_{\tau}^{2\tau}\tau\mathe^{-\mathi\omega t}\D{t} \\
        & = \left.\frac{(1 +\mathi\omega t)\mathe^{-\mathi\omega t}}{\omega^2}\right|_{0}^{\tau} + \left.\frac{\tau\mathe^{-\mathi\omega t}}{-\mathi\omega}\right|_{\tau}^{2\tau} \\
        & = \frac{1 + \mathi\omega\tau}{\omega^2}\mathe^{-\mathi\omega\tau} - \frac{1}{\omega^2} + \frac{\tau\mathe^{-2\mathi\omega\tau}}{-\mathi\omega} - \frac{\tau\mathe^{-\mathi\omega\tau}}{-\mathi\omega} \\
        & = \frac{1 + \mathi\omega\tau}{\omega^2}\mathe^{-\mathi\omega\tau} - \frac{1}{\omega^2} + \frac{\mathi\tau}{\omega}\mathe^{-2\mathi\omega \tau} - \frac{\mathi\tau}{\omega}\mathe^{-\mathi \omega \tau} \\
        & = \frac{\mathi\tau}{\omega}\mathe^{-2\mathi\omega\tau} + \frac{1}{\omega^2}\mathe^{-\mathi\omega\tau} - \frac{1}{\omega^2}.
    \end{align*}
    因此，$f(t)$ 的傅里叶变换为
    \begin{align*}
        F(\omega) = \frac{\mathi\tau}{\omega}\mathe^{-2\mathi\omega\tau} + \frac{1}{\omega^2}\mathe^{-\mathi\omega\tau} - \frac{1}{\omega^2}.
    \end{align*}
\end{solution}
